minor: added a lemma for builtin calls

common/Events.v
@@ -673,6 +673,11 @@ Record extcall_properties (sem: extcall_sem) (sg: signature) : Prop :=
     sem ge vargs m1 t vres m2 ->
     Mem.valid_block m1 b -> Mem.valid_block m2 b;
 
+  ec_tid:
+    forall ge vargs m1 t vres m2,
+    sem ge vargs m1 t vres m2 ->
+    Mem.tid (Mem.support m1) = Mem.tid (Mem.support m2);
+
 (** External calls cannot increase the max permissions of a valid block.
     They can decrease the max permissions, e.g. by freeing. *)
   ec_max_perm:
@@ -810,6 +815,7 @@ Proof.
 (* max perms *)
 - inv H; auto.
 (* readonly *)
+- inv H; auto.
 - inv H; auto.
 (* mem extends *)
 - inv H. inv H1. inv H6. inv H4.
@@ -960,6 +966,7 @@ Proof.
 - unfold proj_sig_res; simpl. inv H; constructor.
 (* valid block *)
 - inv H. inv H1. auto. eauto with mem.
+- inv H. inv H0. auto. erewrite <- Mem.support_store; eauto.
 (* perms *)
 - inv H. inv H2. auto. eauto with mem.
 (* readonly *)
@@ -1036,6 +1043,8 @@ Proof.
 - inv H. simpl. unfold Tptr; destruct Archi.ptr64; auto.
 (* valid block *)
 - inv H. eauto with mem.
+- inv H. apply Mem.support_alloc in H0. apply Mem.support_store in H1.
+  rewrite H1, H0. reflexivity.
 (* perms *)
 - inv H. exploit Mem.perm_alloc_inv. eauto. eapply Mem.perm_store_2; eauto.
   rewrite dec_eq_false. auto.
@@ -1122,6 +1131,7 @@ Proof.
 - inv H; simpl; auto.
 (* valid block *)
 - inv H; eauto with mem.
+- inv H. erewrite <- Mem.support_free; eauto. auto.
 (* perms *)
 - inv H; eauto using Mem.perm_free_3.
 (* readonly *)
@@ -1242,6 +1252,7 @@ Proof.
   intros. inv H. exact I.
 - (* valid blocks *)
   intros. inv H. eauto with mem.
+- intros. inv H. erewrite <- Mem.support_storebytes; eauto.
 - (* perms *)
   intros. inv H. eapply Mem.perm_storebytes_2; eauto.
 - (* readonly *)
@@ -1367,6 +1378,7 @@ Proof.
 - inv H; auto.
 (* perms *)
 - inv H; auto.
+- inv H; auto.
 (* readonly *)
 - inv H; auto.
 (* mem extends *)
@@ -1413,6 +1425,7 @@ Proof.
 - inv H; auto.
 (* perms *)
 - inv H; auto.
+- inv H; auto.
 (* readonly *)
 - inv H; auto.
 (* mem extends *)
@@ -1455,6 +1468,7 @@ Proof.
 (* well typed *)
 - inv H. simpl. auto.
 (* valid blocks *)
+- inv H; auto.
 - inv H; auto.
 (* perms *)
 - inv H; auto.
@@ -1506,6 +1520,7 @@ Proof.
 (* valid blocks *)
 - inv H; auto.
 (* perms *)
+- inv H; auto.
 - inv H; auto.
 (* readonly *)
 - inv H; auto.
@@ -1622,6 +1637,7 @@ Qed.
 
 Definition external_call_well_typed_gen ef := ec_well_typed (external_call_spec ef).
 Definition external_call_valid_block ef := ec_valid_block (external_call_spec ef).
+Definition external_call_tid ef := ec_tid (external_call_spec ef).
 Definition external_call_max_perm ef := ec_max_perm (external_call_spec ef).
 Definition external_call_readonly ef := ec_readonly (external_call_spec ef).
 Definition external_call_mem_extends ef := ec_mem_extends (external_call_spec ef).
